backend/CminorSel.v
@@ -137,21 +137,21 @@ Inductive state: Type :=
              (sp: val)                  (**r current stack pointer *)
              (e: env)                   (**r current local environment *)
              (m: mem)                   (**r current memory state *)
-             (st: stree),
+             (st: struc),
       state
   | Callstate:                          (**r invocation of a fundef  *)
       forall (f: fundef)                (**r fundef to invoke *)
              (args: list val)           (**r arguments provided by caller *)
              (k: cont)                  (**r what to do next  *)
              (m: mem)                   (**r memory state *)
-             (st:stree)
+             (st: struc)
              (id: ident),
       state
   | Returnstate:
       forall (v: val)                   (**r return value *)
              (k: cont)                  (**r what to do next *)
              (m: mem)                   (**r memory state *)
-             (st:stree),
+             (st: struc),
       state.
 
 Section RELSEM.
@@ -344,10 +344,10 @@ Inductive step: state -> trace -> state -> Prop :=
   | step_skip_block: forall f k sp e m st,
       step (State f Sskip (Kblock k) sp e m st)
         E0 (State f Sskip k sp e m st)
-  | step_skip_call: forall f k sp e m m' st st' p,
+  | step_skip_call: forall f k sp e m m' st st',
       is_call_cont k ->
       Mem.free m sp 0 f.(fn_stackspace) = Some m' ->
-      return_stree st  = Some (st',p) ->
+      struc_return_frame st = Some st' ->
       step (State f Sskip k (Vptr sp Ptrofs.zero) e m st)
         E0 (Returnstate Vundef k m' st')
 
@@ -373,14 +373,14 @@ Inductive step: state -> trace -> state -> Prop :=
       step (State f (Scall optid sig a bl) k sp e m st)
         E0 (Callstate fd vargs (Kcall optid f sp e k) m st id)
 
-  | step_tailcall: forall f sig a bl k sp e m vf vargs fd m' st st' p id,
+  | step_tailcall: forall f sig a bl k sp e m vf vargs fd m' st st' id,
       vf = Vptr (Global id) (Ptrofs.zero) ->
       eval_expr_or_symbol (Vptr sp Ptrofs.zero) e m nil a vf ->
       eval_exprlist (Vptr sp Ptrofs.zero) e m nil bl vargs ->
       Genv.find_funct ge vf = Some fd ->
       funsig fd = sig ->
       Mem.free m sp 0 f.(fn_stackspace) = Some m' ->
-      return_stree st  = Some (st',p) ->
+      struc_return_frame st  = Some st' ->
       step (State f (Stailcall sig a bl) k (Vptr sp Ptrofs.zero) e m st)
         E0 (Callstate fd vargs (call_cont k) m' st' id)
 
@@ -422,16 +422,16 @@ Inductive step: state -> trace -> state -> Prop :=
       step (State f (Sswitch a) k sp e m st)
         E0 (State f (Sexit n) k sp e m st)
 
-  | step_return_0: forall f k sp e m m' st st' p,
+  | step_return_0: forall f k sp e m m' st st',
       Mem.free m sp 0 f.(fn_stackspace) = Some m' ->
-      return_stree st = Some (st',p) ->
+      struc_return_frame st = Some st' ->
       step (State f (Sreturn None) k (Vptr sp Ptrofs.zero) e m st)
         E0 (Returnstate Vundef (call_cont k) m' st')
 
-  | step_return_1: forall f a k sp e m v m' st st' p,
+  | step_return_1: forall f a k sp e m v m' st st',
       eval_expr (Vptr sp Ptrofs.zero) e m nil a v ->
       Mem.free m sp 0 f.(fn_stackspace) = Some m' ->
-      return_stree st = Some (st',p) ->
+      struc_return_frame st = Some st' ->
       step (State f (Sreturn (Some a)) k (Vptr sp Ptrofs.zero) e m st)
         E0 (Returnstate v (call_cont k) m' st')
 
@@ -444,9 +444,9 @@ Inductive step: state -> trace -> state -> Prop :=
       step (State f (Sgoto lbl) k sp e m st)
         E0 (State f s' k' sp e m st)
 
-  | step_internal_function: forall f vargs k m m' sp st st' st'' e id path,
-      next_stree st id = (st',path) ->
-      next_block_stree' st' = (sp,st'') ->
+  | step_internal_function: forall f vargs k m m' sp st st' st'' e id,
+      struc_incr_frame st id = st' ->
+      struc_alloc_stack st' = (st'',sp) ->
       Mem.alloc m 0 f.(fn_stackspace) sp = Some m' ->
       set_locals f.(fn_vars) (set_params vargs f.(fn_params)) = e ->
       step (Callstate (Internal f) vargs k m st id)
@@ -466,11 +466,12 @@ End RELSEM.
 Inductive initial_state (p: program): state -> Prop :=
   | initial_state_intro: forall b f m0,
       let ge := Genv.globalenv p in
+      let st := Genv.init_struc p in
       Genv.init_mem p = Some m0 ->
       Genv.find_symbol ge p.(prog_main) = Some b ->
       Genv.find_funct_ptr ge b = Some f ->
       funsig f = signature_main ->
-      initial_state p (Callstate f nil Kstop m0 empty_stree p.(prog_main)).
+      initial_state p (Callstate f nil Kstop m0 st p.(prog_main)).
 
 Inductive final_state: state -> int -> Prop :=
   | final_state_intro: forall r m st,
