common/Switch.v
@@ -23,7 +23,7 @@ Require Import Maps.
 Require Import Integers.
 Require Import Values.
 Require Import Memstructure.
-Import StrucMem.
+Import Mem.
 
 (** A multi-way branch is composed of a list of (key, action) pairs,
   plus a default action.  *)
